Update MatchActionRule to Transformer.
That was surprisingly easy.
Guess equivalence checker and ir-to-smt translation are quite decoupled.

SmtQuery.v
@@ -272,13 +272,13 @@ Qed.
 
 Definition equivalence_checker
   (s : ProgramState SmtArithExpr)
-  (sr1 : MatchActionRule) (sr2 : MatchActionRule)
+  (t1 : Transformer) (t2 : Transformer)
   (header_list : list Header) (state_var_list : list StateVar)
    :  SmtResult :=
   (* assume a starting symbolic state s*)
-  (* convert sr1 and sr2 to an equivalent final SmtArithExpr, assuming a start state of s *)
-  let s1 := eval_match_action_rule_smt sr1 s in
-  let s2 := eval_match_action_rule_smt sr2 s in
+  (* convert t1 and t2 to an equivalent final SmtArithExpr, assuming a start state of s *)
+  let s1 := eval_transformer_smt t1 s in
+  let s2 := eval_transformer_smt t2 s in
   (* check if the headers and state vars are equivalent *)
   smt_query (check_headers_and_state_vars s1 s2 header_list state_var_list).
 
@@ -349,50 +349,50 @@ Proof.
 Qed.
 
 Lemma eval_smt_bool_lemma_hdr :
-  forall sr1 sr2 s h f,
+  forall t1 t2 s h f,
   eval_smt_bool
-(SmtBoolEq (header_map (eval_match_action_rule_smt sr1 s) h)
-(header_map (eval_match_action_rule_smt sr2 s) h)) f = true ->
-header_map (eval_match_action_rule_uint8 sr1 (eval_sym_state s f)) h =
-header_map (eval_match_action_rule_uint8 sr2 (eval_sym_state s f)) h.
+(SmtBoolEq (header_map (eval_transformer_smt t1 s) h)
+(header_map (eval_transformer_smt t2 s) h)) f = true ->
+header_map (eval_transformer_uint8 t1 (eval_sym_state s f)) h =
+header_map (eval_transformer_uint8 t2 (eval_sym_state s f)) h.
 Proof.
-  intros sr1 sr2 s h f.
+  intros t1 t2 s h f.
   intro H.
   apply smt_bool_eq_true in H.
-  rewrite commute_sym_vs_conc_ma_rule.
-  rewrite commute_sym_vs_conc_ma_rule.
+  rewrite commute_sym_vs_conc_transfomer.
+  rewrite commute_sym_vs_conc_transfomer.
   apply H.
 Qed.
 
 Lemma eval_smt_bool_lemma_state :
-  forall sr1 sr2 s sv f,
+  forall t1 t2 s sv f,
   eval_smt_bool
-(SmtBoolEq (state_var_map (eval_match_action_rule_smt sr1 s) sv)
-(state_var_map (eval_match_action_rule_smt sr2 s) sv)) f = true ->
-state_var_map (eval_match_action_rule_uint8 sr1 (eval_sym_state s f)) sv =
-state_var_map (eval_match_action_rule_uint8 sr2 (eval_sym_state s f)) sv.
+(SmtBoolEq (state_var_map (eval_transformer_smt t1 s) sv)
+(state_var_map (eval_transformer_smt t2 s) sv)) f = true ->
+state_var_map (eval_transformer_uint8 t1 (eval_sym_state s f)) sv =
+state_var_map (eval_transformer_uint8 t2 (eval_sym_state s f)) sv.
 Proof.
-  intros sr1 sr2 s sv f.
+  intros t1 t2 s sv f.
   intro H.
   apply smt_bool_eq_true in H.
-  rewrite commute_sym_vs_conc_ma_rule.
-  rewrite commute_sym_vs_conc_ma_rule.
+  rewrite commute_sym_vs_conc_transfomer.
+  rewrite commute_sym_vs_conc_transfomer.
   apply H.
 Qed.
 
 (* Soundness lemma about equivalence_checker conditional on the axioms above *)
 Lemma equivalence_checker_sound :
-  forall s sr1 sr2 header_list state_var_list f,
-  equivalence_checker s sr1 sr2 header_list state_var_list = SmtUnsat ->
+  forall s t1 t2 header_list state_var_list f,
+  equivalence_checker s t1 t2 header_list state_var_list = SmtUnsat ->
   let c  := eval_sym_state s f in
-  let c1 := eval_match_action_rule_uint8 sr1 c in
-  let c2 := eval_match_action_rule_uint8 sr2 c in
+  let c1 := eval_transformer_uint8 t1 c in
+  let c2 := eval_transformer_uint8 t2 c in
   (forall v, In v header_list ->
   (header_map c1 v) = (header_map c2 v)) /\
   (forall v, In v state_var_list ->
   (state_var_map c1 v) = (state_var_map c2 v)).
 Proof.
-  intros s sr1 sr2 header_list state_var_list f.
+  intros s t1 t2 header_list state_var_list f.
   intro H.
   simpl.
   unfold equivalence_checker in H.
@@ -425,54 +425,54 @@ Proof.
 Qed.
 
 Lemma eval_smt_bool_lemma_hdr_false :
-  forall sr1 sr2 s h f,
+  forall t1 t2 s h f,
   eval_smt_bool
-(SmtBoolEq (header_map  (eval_match_action_rule_smt sr1 s) h)
-(header_map  (eval_match_action_rule_smt sr2 s) h)) f = false ->
-header_map (eval_match_action_rule_uint8 sr1 (eval_sym_state s f)) h <>
-header_map (eval_match_action_rule_uint8 sr2 (eval_sym_state s f)) h.
+(SmtBoolEq (header_map  (eval_transformer_smt t1 s) h)
+(header_map  (eval_transformer_smt t2 s) h)) f = false ->
+header_map (eval_transformer_uint8 t1 (eval_sym_state s f)) h <>
+header_map (eval_transformer_uint8 t2 (eval_sym_state s f)) h.
 Proof.
-  intros sr1 sr2 s h f.
+  intros t1 t2 s h f.
   intro H.
   apply smt_bool_eq_false in H.
-  rewrite commute_sym_vs_conc_ma_rule.
-  rewrite commute_sym_vs_conc_ma_rule.
+  rewrite commute_sym_vs_conc_transfomer.
+  rewrite commute_sym_vs_conc_transfomer.
   apply H.
 Qed.
 
 Lemma eval_smt_bool_lemma_state_false :
-  forall sr1 sr2 s sv f,
+  forall t1 t2 s sv f,
   eval_smt_bool
-(SmtBoolEq (state_var_map  (eval_match_action_rule_smt sr1 s) sv)
-(state_var_map  (eval_match_action_rule_smt sr2 s) sv)) f = false ->
-state_var_map (eval_match_action_rule_uint8 sr1 (eval_sym_state s f)) sv <>
-state_var_map (eval_match_action_rule_uint8 sr2 (eval_sym_state s f)) sv.
+(SmtBoolEq (state_var_map  (eval_transformer_smt t1 s) sv)
+(state_var_map  (eval_transformer_smt t2 s) sv)) f = false ->
+state_var_map (eval_transformer_uint8 t1 (eval_sym_state s f)) sv <>
+state_var_map (eval_transformer_uint8 t2 (eval_sym_state s f)) sv.
 Proof.
-  intros sr1 sr2 s sv f.
+  intros t1 t2 s sv f.
   intro H.
   apply smt_bool_eq_false in H.
-  rewrite commute_sym_vs_conc_ma_rule.
-  rewrite commute_sym_vs_conc_ma_rule.
+  rewrite commute_sym_vs_conc_transfomer.
+  rewrite commute_sym_vs_conc_transfomer.
   apply H.
 Qed.
 
 (* Completeness lemma about equivalence_checker conditional on the axioms above *)
 Lemma equivalence_checker_complete :
-  forall s sr1 sr2 header_list state_var_list f',
-  equivalence_checker s sr1 sr2 header_list state_var_list = SmtSat f' ->
+  forall s t1 t2 header_list state_var_list f',
+  equivalence_checker s t1 t2 header_list state_var_list = SmtSat f' ->
   let c' := eval_sym_state s f' in
-  let c1 := eval_match_action_rule_uint8 sr1 c' in
-  let c2 := eval_match_action_rule_uint8 sr2 c' in
+  let c1 := eval_transformer_uint8 t1 c' in
+  let c2 := eval_transformer_uint8 t2 c' in
   (exists v, In v header_list /\
   (header_map c1 v) <> (header_map c2 v)) \/
   (exists v, In v state_var_list /\
   (state_var_map c1 v) <> (state_var_map c2 v)).
 Proof.
-  intros s sr1 sr2 header_list state_var_list f'.
+  intros s t1 t2 header_list state_var_list f'.
   intro H.
   simpl.
   unfold equivalence_checker in H.
-  destruct (smt_query (check_headers_and_state_vars (eval_match_action_rule_smt sr1 s) (eval_match_action_rule_smt sr2 s) header_list state_var_list)) eqn:H_query.
+  destruct (smt_query (check_headers_and_state_vars (eval_transformer_smt t1 s) (eval_transformer_smt t2 s) header_list state_var_list)) eqn:H_query.
   - injection H as Heq.
     subst f'.
     apply smt_query_sound_some in H_query.
@@ -480,13 +480,13 @@ Proof.
     destruct H_query as [H_header | H_state_var].
     -- destruct H_header as [h Hw].
        destruct Hw.
-       pose proof (eval_smt_bool_lemma_hdr_false sr1 sr2 s h f H0) as H_neq.
+       pose proof (eval_smt_bool_lemma_hdr_false t1 t2 s h f H0) as H_neq.
        left.
        exists h.
        split; assumption.
     -- destruct H_state_var as [sv Hw].
        destruct Hw.
-       pose proof (eval_smt_bool_lemma_state_false sr1 sr2 s sv f H0) as H_neq.
+       pose proof (eval_smt_bool_lemma_state_false t1 t2 s sv f H0) as H_neq.
        right.
        exists sv.
        split; assumption.
